fairness/lawyer/examples/obls_tactics.v
@@ -6,7 +6,7 @@ From iris.algebra Require Import auth gmap gset excl excl_auth csum mono_nat.
 From iris.base_logic.lib Require Import invariants.
 From trillium.program_logic Require Export weakestpre adequacy ectx_lifting.
 From trillium.fairness Require Import utils.
-From trillium.fairness.lawyer.obligations Require Import obligations_model obligations_resources obligations_am obligations_em obligations_logic.
+From trillium.fairness.lawyer.obligations Require Import obligations_model obligations_resources obligations_am obligations_em obligations_logic env_helpers.
 From trillium.fairness.lawyer Require Import sub_action_em.
 From trillium.fairness.lawyer Require Import program_logic.
 
@@ -24,22 +24,17 @@ Ltac BOU_burn_cp :=
 
 Ltac MU_by_BOU :=
   try iNext;
-  match goal with
-  | [OB_AMU: AMU_lift_MU _ _ _ _ _ |- envs_entails _ (MU _ _ _) ] =>
-      iApply OB_AMU; [(try rewrite nclose_nroot); done| ];
-      iApply BOU_AMU
-  end.
+  iApply ohe_obls_AMU; [(try rewrite nclose_nroot); done| ];  
+  iApply BOU_AMU
+.
 
 Ltac MU_by_burn_cp := MU_by_BOU; BOU_burn_cp.
 
 Ltac MU__f_by_BOU R' :=
   try iNext;
-  match goal with
-  | [OBLS_AMU__f: forall τ, @AMU_lift_MU__f _ _ _ _ _ _ _ _ _ |-
-                       envs_entails _ (MU__f _ _ _ _) ] =>
-      iApply OBLS_AMU__f; [(try rewrite nclose_nroot); done| ];
-      iApply (BOU_AMU__f' _ _ _ _ _ R')
-  end.
+  iApply ohe_obls_AMU__f; [(try rewrite nclose_nroot); done| ];
+  iApply (BOU_AMU__f' _ _ _ _ _ R')
+.
 
 Ltac pure_step_hl :=
   iApply sswp_MU_wp; [done| ];
@@ -53,4 +48,3 @@ Ltac pure_steps := repeat (pure_step_cases; []).
 Ltac split_cps cps_res n :=
   let fmt := constr:(("[" ++ cps_res ++ "' " ++ cps_res ++ "]")%string) in
   iDestruct (cp_mul_split' _ _ n with cps_res) as fmt; [lia| ].
-
