fairness/lawyer/examples/ticketlock/fair_lock.v
@@ -1,7 +1,187 @@
 From trillium.fairness.lawyer.examples Require Import obls_atomic.
 From trillium.fairness.lawyer.obligations Require Import obligations_model  obligations_am obligations_em obligations_logic.
 From trillium.fairness.lawyer Require Import sub_action_em program_logic.
-From trillium.fairness.lawyer.obligations Require Import obligations_resources.
+From trillium.fairness.lawyer.obligations Require Import obligations_resources env_helpers.
+
+
+(* Section FairLockSpec. *)
+
+(*   Definition FL_st: Type := val * nat * bool. *)
+
+(*   Definition fl_round: FL_st -> nat := fun '(_, r, _) => r.  *)
+
+(*   Context `{OfeDiscrete DegO} `{OfeDiscrete LevelO}. *)
+(*   Context `{@LeibnizEquiv (ofe_car LevelO) (ofe_equiv LevelO)}.  *)
+  
+(*   Let Degree := ofe_car DegO. *)
+(*   Let Level := ofe_car LevelO. *)
+
+(*   Context `{OPRE: ObligationsParamsPre Degree Level LIM_STEPS}. *)
+(*   Let OP := LocaleOP (Locale := locale heap_lang). *)
+(*   Existing Instance OP. *)
+(*   Let OM := ObligationsModel. *)
+  
+(*   Record FairLockPre := { *)
+(*     fl_c__cr: nat; fl_B: nat -> nat; *)
+(*     fl_GpreS :> gFunctors -> Set; *)
+(*     fl_GS :> gFunctors -> Set; *)
+(*     fl_LK {Σ: gFunctors} {FLG: fl_GS Σ} {HEAP: gen_heapGS loc val Σ}: FL_st -> iProp Σ; *)
+(*     fl_d__h: Degree; *)
+(*     fl_d__l: Degree; *)
+(*     fl_d__m: Degree; *)
+(*     fl_degs_lh: deg_lt fl_d__l fl_d__h; *)
+(*     fl_degs_hm: deg_lt fl_d__h fl_d__m; *)
+(*     fl_acq_lvls: gset Level;                                      *)
+(*     fl_create: val; fl_acquire: val; fl_release: val; *)
+(*   }. *)
+
+(*   Definition fl_ι: namespace := nroot .@ "fair_lock". *)
+
+(*   Context {Σ: gFunctors}. *)
+  
+(*   Let OAM := ObligationsAM.  *)
+(*   Let ASEM := ObligationsASEM. *)
+(*   (* Keeping the more general interface for future developments *) *)
+(*   Context `{oGS': @asem_GS _ _ ASEM Σ}. *)
+(*   Let oGS: ObligationsGS (OP := OP) Σ := oGS'. *)
+(*   Existing Instance oGS. *)
+  
+(*   Context `{EM: ExecutionModel heap_lang M}. *)
+(*   Context `{hGS: @heapGS Σ _ EM}. *)
+(*   Let eGS: em_GS Σ := heap_fairnessGS (heapGS := hGS). *)
+  
+(*   Context {FLP: FairLockPre}. *)
+
+(*   Definition TAU_FL τ P Q L c π q Φ O fg: iProp Σ :=   *)
+(*     TAU τ P Q L c (⊤ ∖ ↑fl_ι) π q Φ O fg (ST := FL_st) (oGS' := oGS'). *)
+
+(*   (* Definition TAU_FL τ P Q L (* TGT *) c π q *) *)
+(*   (*   Φ *) *)
+(*   (*   O *) *)
+(*   (*   fg: iProp Σ :=  *) *)
+(*   (*   TAU τ P Q L (* fl_round *) *) *)
+(*   (*     (* TGT *) *) *)
+(*   (*     (* (fl_d__h FLP) (fl_d__l FLP) *) *) *)
+(*   (*     c *) *)
+(*   (*     (⊤ ∖ ↑fl_ι) *) *)
+(*   (*     π q *) *)
+(*   (*     Φ *) *)
+(*   (*     O *) *)
+(*   (*     (* RR *) *) *)
+(*   (*     (* (fl_FG_RR RR π) *) *) *)
+(*   (*     fg *) *)
+(*   (*     (oGS' := oGS'). *) *)
+  
+(*   Definition acq_FG_RR (RR: option nat -> iProp Σ) π: AbortClause (ST := FL_st) := *)
+(*     AC_RR (fl_d__l FLP) π *)
+(*       (fun '(_, n, _) => n) (fun '(_, _, b) => (⌜ b = true ⌝)%I) *)
+(*       RR (fl_d__h FLP) (oGS' := oGS'). *)
+  
+(*   Definition TLAT_FL τ P Q L (* TGT *) fg (POST: FL_st -> FL_st -> option (iProp Σ)) *)
+(*     get_ret c e : iProp Σ :=  *)
+(*     TLAT τ P Q L *)
+(*       (* fl_round *) *)
+(*       (* TGT *) *)
+(*       (* (fl_d__h FLP) (fl_d__l FLP) (fl_d__m FLP) *) *)
+(*       (fl_d__m FLP) *)
+(*       c (fl_B FLP) *)
+(*       (↑ fl_ι) e NotStuck *)
+(*       (* (fl_d__h FLP) (fl_d__l FLP)  *) *)
+(*       fg *)
+(*       POST *)
+(*       get_ret *)
+(*       (oGS' := oGS'). *)
+  
+(*   Definition TLAT_FL_RR τ P Q L TGT (POST: FL_st -> FL_st -> option (iProp Σ)) *)
+(*     get_ret c e : iProp Σ :=  *)
+(*     TLAT_RR τ P Q L *)
+(*       (fl_d__m FLP)  *)
+(*       c (fl_B FLP) *)
+(*       (↑ fl_ι) e NotStuck *)
+(*       (fl_d__h FLP) (fl_d__l FLP) *)
+(*       fl_round *)
+(*       TGT *)
+(*       POST *)
+(*       get_ret *)
+(*       (oGS' := oGS'). *)
+  
+(*   Definition acquire_at_pre {FLG: fl_GS FLP Σ} (lk: val) (x: FL_st): iProp Σ := *)
+(*     ▷ fl_LK FLP x (FLG := FLG) ∗ ⌜ x.1.1 = lk ⌝.  *)
+(*   Definition acquire_at_post {FLG: fl_GS FLP Σ} (lk: val) (y x: FL_st): iProp Σ := *)
+(*     fl_LK FLP y (FLG := FLG) ∗ ⌜ y.1 = x.1 /\ x.2 = false /\ y.2 = true⌝. *)
+(*   Definition release_at_pre {FLG: fl_GS FLP Σ} (lk: val) (x: FL_st): iProp Σ := *)
+(*     ▷ fl_LK FLP x (FLG := FLG) ∗ ⌜ x.2 = true /\ x.1.1 = lk⌝.  *)
+(*   Definition release_at_post {FLG: fl_GS FLP Σ} (lk: val) (y x: FL_st): iProp Σ := *)
+(*     fl_LK FLP y (FLG := FLG) ∗ ⌜ y.1.2 = (x.1.2 + 1)%nat /\ y.2 = false /\ y.1.1 = x.1.1 ⌝. *)
+    
+(* End FairLockSpec. *)
+
+
+(* Section FairLockDef. *)
+
+(*   Context `{OfeDiscrete DegO} `{OfeDiscrete LevelO}. *)
+(*   Context `{@LeibnizEquiv (ofe_car LevelO) (ofe_equiv LevelO)}.  *)
+  
+(*   Let Degree := ofe_car DegO. *)
+(*   Let Level := ofe_car LevelO. *)
+
+(*   Context `{OPRE: ObligationsParamsPre Degree Level LIM_STEPS}. *)
+(*   Let OP := LocaleOP (Locale := locale heap_lang). *)
+(*   Existing Instance OP. *)
+(*   Let OM := ObligationsModel. *)
+
+(*   Context {FLP: FairLockPre}. *)
+
+(*   Record FairLock := {     *)
+
+(*     fl_is_lock `{FLG: fl_GS FLP Σ} {HEAP: gen_heapGS loc val Σ} *)
+(*       (ASEM := ObligationsASEM) {oGS': @asem_GS _ _ ASEM Σ}: val -> nat -> iProp Σ; *)
+(*     fl_is_lock_pers {Σ} {FLG: fl_GS FLP Σ} {HEAP: gen_heapGS loc val Σ} *)
+(*       (ASEM := ObligationsASEM) {oGS': @asem_GS _ _ ASEM Σ} *)
+(*       lk c :: Persistent (fl_is_lock lk c (FLG := FLG) (oGS' := oGS')); *)
+
+(*     fl_release_token `{FLG: fl_GS FLP Σ}: iProp Σ; *)
+
+(*     fl_create_spec {Σ} {FLG_PRE: fl_GpreS FLP Σ} *)
+(*         (ASEM := ObligationsASEM) {oGS': @asem_GS _ _ ASEM Σ} `{EM: ExecutionModel heap_lang M} {hGS : heapGS Σ EM} *)
+(*       (oGS: ObligationsGS (OP := OP) Σ := oGS'): *)
+(*       ⊢ ⌜ fl_c__cr FLP <= LIM_STEPS ⌝ -∗ ∀ τ π c, *)
+(*         {{{ cp π (fl_d__m FLP) ∗ th_phase_eq τ π }}} *)
+(*             fl_create FLP #() @ τ *)
+(*         {{{ lk, RET lk; ∃ FLG: fl_GS FLP Σ, fl_LK _ (lk, 0, false) (FLG := FLG) ∗ fl_is_lock lk c (FLG := FLG) (oGS' := oGS') ∗ th_phase_eq τ π }}}; *)
+
+(*     fl_acquire_spec {Σ} {FLG: fl_GS FLP Σ} *)
+(*         (ASEM := ObligationsASEM) {oGS': @asem_GS _ _ ASEM Σ} `{EM: ExecutionModel heap_lang M} {hGS : heapGS Σ EM} *)
+(*       (oGS: ObligationsGS (OP := OP) Σ := oGS') *)
+(*       (lk: val) c τ: *)
+(*       (fl_is_lock (FLG := FLG) (oGS' := oGS')) lk c ⊢ *)
+(*         TLAT_FL_RR τ *)
+(*         (acquire_at_pre lk (FLG := FLG)) *)
+(*         (acquire_at_post lk (FLG := FLG)) *)
+(*         (fl_acq_lvls FLP) *)
+(*         (fun '(_, _, b) => ⌜ b = true ⌝) *)
+(*         (fun _ _ => Some $ fl_release_token (FLG := FLG)) *)
+(*         (fun _ _ => #()) *)
+(*         c (fl_acquire FLP lk) *)
+(*         (oGS' := oGS') (FLP := FLP); *)
+                                     
+(*     fl_release_spec {Σ} {FLG: fl_GS FLP Σ} *)
+(*         (ASEM := ObligationsASEM) {oGS': @asem_GS _ _ ASEM Σ} `{EM: ExecutionModel heap_lang M} {hGS : heapGS Σ EM} *)
+(*       (oGS: ObligationsGS (OP := OP) Σ := oGS') *)
+(*       (lk: val) c τ: (fl_is_lock (FLG := FLG) (oGS' := oGS')) lk c ∗ fl_release_token (FLG := FLG) ⊢ *)
+(*         TLAT_FL τ *)
+(*         (release_at_pre lk (FLG := FLG)) *)
+(*         (release_at_post lk (FLG := FLG)) *)
+(*         ∅ *)
+(*         (* (fun _ => True%type) *) *)
+(*         AC_none *)
+(*         (fun _ _ => None) *)
+(*         (fun _ '(_, r, _) => #r) *)
+(*         c (fl_release FLP lk) *)
+(*         (oGS' := oGS') (FLP := FLP); *)
+(*   }. *)
+
+(* End FairLockDef. *)
 
 
 Section FairLockSpec.
@@ -10,87 +190,62 @@ Section FairLockSpec.
 
   Definition fl_round: FL_st -> nat := fun '(_, r, _) => r. 
 
-  Context `{OfeDiscrete DegO} `{OfeDiscrete LevelO}.
-  Context `{@LeibnizEquiv (ofe_car LevelO) (ofe_equiv LevelO)}. 
-  
-  Let Degree := ofe_car DegO.
-  Let Level := ofe_car LevelO.
+  Context `{OP: OP_HL DegO LvlO LIM_STEPS}.
+  Existing Instance om_hl_OP.
+  Notation "'Degree'" := (om_hl_Degree). 
+  Notation "'Level'" := (om_hl_Level).
+  Context `{EM: ExecutionModel heap_lang M}.
 
-  Context `{OPRE: ObligationsParamsPre Degree Level LIM_STEPS}.
-  Let OP := LocaleOP (Locale := locale heap_lang).
-  Existing Instance OP.
-  Let OM := ObligationsModel.
   
   Record FairLockPre := {
     fl_c__cr: nat; fl_B: nat -> nat;
-    fl_GpreS :> gFunctors -> Set;
-    fl_GS :> gFunctors -> Set;
-    fl_LK {Σ: gFunctors} {FLG: fl_GS Σ} {HEAP: gen_heapGS loc val Σ}: FL_st -> iProp Σ;
+    fl_GpreS : gFunctors -> Set;
+    fl_GS : gFunctors -> Set;
+    fl_LK `{FLG: fl_GS Σ} {OHE: OM_HL_Env OP EM Σ}: FL_st -> iProp Σ;
     fl_d__h: Degree;
     fl_d__l: Degree;
     fl_d__m: Degree;
     fl_degs_lh: deg_lt fl_d__l fl_d__h;
     fl_degs_hm: deg_lt fl_d__h fl_d__m;
-    fl_acq_lvls: gset Level;                                     
+    fl_acq_lvls: gset Level;
     fl_create: val; fl_acquire: val; fl_release: val;
   }.
 
   Definition fl_ι: namespace := nroot .@ "fair_lock".
 
   Context {Σ: gFunctors}.
+  Context {OHE: OM_HL_Env OP EM Σ}.
   
-  Let OAM := ObligationsAM. 
-  Let ASEM := ObligationsASEM.
-  (* Keeping the more general interface for future developments *)
-  Context `{oGS': @asem_GS _ _ ASEM Σ}.
-  Let oGS: ObligationsGS (OP := OP) Σ := oGS'.
-  Existing Instance oGS.
+  (* Let OAM := ObligationsAM.  *)
+  (* Let ASEM := ObligationsASEM. *)
+  (* (* Keeping the more general interface for future developments *) *)
+  (* Context `{oGS': @asem_GS _ _ ASEM Σ}. *)
+  (* Let oGS: ObligationsGS (OP := OP) Σ := oGS'. *)
+  (* Existing Instance ohe_oGS'. *)
   
-  Context `{EM: ExecutionModel heap_lang M}.
-  Context `{hGS: @heapGS Σ _ EM}.
-  Let eGS: em_GS Σ := heap_fairnessGS (heapGS := hGS).
+  (* Context `{hGS: @heapGS Σ _ EM}. *)
+  (* Let eGS: em_GS Σ := heap_fairnessGS (heapGS := hGS). *)
   
   Context {FLP: FairLockPre}.
 
   Definition TAU_FL τ P Q L c π q Φ O fg: iProp Σ :=  
-    TAU τ P Q L c (⊤ ∖ ↑fl_ι) π q Φ O fg (ST := FL_st) (oGS' := oGS').
+    TAU τ P Q L c (⊤ ∖ ↑fl_ι) π q Φ O fg (ST := FL_st) (oGS' := ohe_oGS').
 
-  (* Definition TAU_FL τ P Q L (* TGT *) c π q *)
-  (*   Φ *)
-  (*   O *)
-  (*   fg: iProp Σ :=  *)
-  (*   TAU τ P Q L (* fl_round *) *)
-  (*     (* TGT *) *)
-  (*     (* (fl_d__h FLP) (fl_d__l FLP) *) *)
-  (*     c *)
-  (*     (⊤ ∖ ↑fl_ι) *)
-  (*     π q *)
-  (*     Φ *)
-  (*     O *)
-  (*     (* RR *) *)
-  (*     (* (fl_FG_RR RR π) *) *)
-  (*     fg *)
-  (*     (oGS' := oGS'). *)
-  
   Definition acq_FG_RR (RR: option nat -> iProp Σ) π: AbortClause (ST := FL_st) :=
     AC_RR (fl_d__l FLP) π
       (fun '(_, n, _) => n) (fun '(_, _, b) => (⌜ b = true ⌝)%I)
-      RR (fl_d__h FLP) (oGS' := oGS').
+      RR (fl_d__h FLP) (oGS' := ohe_oGS').
   
   Definition TLAT_FL τ P Q L (* TGT *) fg (POST: FL_st -> FL_st -> option (iProp Σ))
     get_ret c e : iProp Σ := 
     TLAT τ P Q L
-      (* fl_round *)
-      (* TGT *)
-      (* (fl_d__h FLP) (fl_d__l FLP) (fl_d__m FLP) *)
       (fl_d__m FLP)
       c (fl_B FLP)
       (↑ fl_ι) e NotStuck
-      (* (fl_d__h FLP) (fl_d__l FLP)  *)
       fg
       POST
       get_ret
-      (oGS' := oGS').
+      (oGS' := ohe_oGS').
   
   Definition TLAT_FL_RR τ P Q L TGT (POST: FL_st -> FL_st -> option (iProp Σ))
     get_ret c e : iProp Σ := 
@@ -103,7 +258,7 @@ Section FairLockSpec.
       TGT
       POST
       get_ret
-      (oGS' := oGS').
+      (oGS' := ohe_oGS').
   
   Definition acquire_at_pre {FLG: fl_GS FLP Σ} (lk: val) (x: FL_st): iProp Σ :=
     ▷ fl_LK FLP x (FLG := FLG) ∗ ⌜ x.1.1 = lk ⌝. 
@@ -115,42 +270,33 @@ Section FairLockSpec.
     fl_LK FLP y (FLG := FLG) ∗ ⌜ y.1.2 = (x.1.2 + 1)%nat /\ y.2 = false /\ y.1.1 = x.1.1 ⌝.
     
 End FairLockSpec.
-
+  
 
 Section FairLockDef.
 
-  Context `{OfeDiscrete DegO} `{OfeDiscrete LevelO}.
-  Context `{@LeibnizEquiv (ofe_car LevelO) (ofe_equiv LevelO)}. 
-  
-  Let Degree := ofe_car DegO.
-  Let Level := ofe_car LevelO.
-
-  Context `{OPRE: ObligationsParamsPre Degree Level LIM_STEPS}.
-  Let OP := LocaleOP (Locale := locale heap_lang).
-  Existing Instance OP.
-  Let OM := ObligationsModel.
-
+  (* Context `{OP: OP_HL DegO LvlO LIM_STEPS}. *)
+  Context {DegO LvlO LIM_STEPS} {OP: OP_HL DegO LvlO LIM_STEPS}.
+  Context `{EM: ExecutionModel heap_lang M}.
   Context {FLP: FairLockPre}.
 
   Record FairLock := {    
 
-    fl_is_lock `{FLG: fl_GS FLP Σ} {HEAP: gen_heapGS loc val Σ}: val -> nat -> iProp Σ;
-    fl_is_lock_pers {Σ} {FLG: fl_GS FLP Σ} {HEAP: gen_heapGS loc val Σ} lk c ::
-      Persistent (fl_is_lock lk c (FLG := FLG));
+    fl_is_lock `{FLG: fl_GS FLP Σ} {OHE: OM_HL_Env OP EM Σ}:
+      val -> nat -> iProp Σ;
+
+    fl_is_lock_pers `{FLG: fl_GS FLP Σ} {OHE: OM_HL_Env OP EM Σ}
+      lk c :: Persistent (fl_is_lock lk c (FLG := FLG));
 
     fl_release_token `{FLG: fl_GS FLP Σ}: iProp Σ;
 
-    fl_create_spec {Σ} {FLG_PRE: fl_GpreS FLP Σ}
-        (ASEM := ObligationsASEM) {oGS': @asem_GS _ _ ASEM Σ} `{EM: ExecutionModel heap_lang M} {hGS : heapGS Σ EM}
-      (oGS: ObligationsGS (OP := OP) Σ := oGS'):
+    fl_create_spec `{FLG_PRE: fl_GpreS FLP Σ} {OHE: OM_HL_Env OP EM Σ}
+      :
       ⊢ ⌜ fl_c__cr FLP <= LIM_STEPS ⌝ -∗ ∀ τ π c,
         {{{ cp π (fl_d__m FLP) ∗ th_phase_eq τ π }}}
             fl_create FLP #() @ τ
         {{{ lk, RET lk; ∃ FLG: fl_GS FLP Σ, fl_LK _ (lk, 0, false) (FLG := FLG) ∗ fl_is_lock lk c (FLG := FLG) ∗ th_phase_eq τ π }}};
 
-    fl_acquire_spec {Σ} {FLG: fl_GS FLP Σ}
-        (ASEM := ObligationsASEM) {oGS': @asem_GS _ _ ASEM Σ} `{EM: ExecutionModel heap_lang M} {hGS : heapGS Σ EM}
-      (oGS: ObligationsGS (OP := OP) Σ := oGS')
+    fl_acquire_spec `{FLG: fl_GS FLP Σ} {OHE: OM_HL_Env OP EM Σ}
       (lk: val) c τ:
       (fl_is_lock (FLG := FLG)) lk c ⊢
         TLAT_FL_RR τ
@@ -161,22 +307,19 @@ Section FairLockDef.
         (fun _ _ => Some $ fl_release_token (FLG := FLG))
         (fun _ _ => #())
         c (fl_acquire FLP lk)
-        (oGS' := oGS') (FLP := FLP);
+        (FLP := FLP);
                                      
-    fl_release_spec {Σ} {FLG: fl_GS FLP Σ}
-        (ASEM := ObligationsASEM) {oGS': @asem_GS _ _ ASEM Σ} `{EM: ExecutionModel heap_lang M} {hGS : heapGS Σ EM}
-      (oGS: ObligationsGS (OP := OP) Σ := oGS')
+    fl_release_spec `{FLG: fl_GS FLP Σ} {OHE: OM_HL_Env OP EM Σ}
       (lk: val) c τ: (fl_is_lock (FLG := FLG)) lk c ∗ fl_release_token (FLG := FLG) ⊢
         TLAT_FL τ
         (release_at_pre lk (FLG := FLG))
         (release_at_post lk (FLG := FLG))
         ∅
-        (* (fun _ => True%type) *)
         AC_none
         (fun _ _ => None)
         (fun _ '(_, r, _) => #r)
         c (fl_release FLP lk)
-        (oGS' := oGS') (FLP := FLP);
+        (FLP := FLP);
   }.
 
 End FairLockDef.
