fairness/lawyer/obligations/env_helpers.v
@@ -1,0 +1,32 @@
+From trillium.fairness.lawyer Require Import sub_action_em.
+From trillium.fairness.lawyer.obligations Require Import obligations_model  obligations_am obligations_em obligations_logic obligations_resources.
+
+
+(* TODO: move all that and use throughout development *)
+
+Class OP_HL (DegO LvlO: ofe) (LIM_STEPS: nat) := {
+    om_hl_DegO_discr :: OfeDiscrete DegO; 
+    om_hl_LvlO_discr :: OfeDiscrete LvlO; 
+    om_hl_LvlO_equiv :: @LeibnizEquiv (ofe_car LvlO) (ofe_equiv LvlO);
+    
+    om_hl_OPRE :: ObligationsParamsPre (ofe_car DegO) (ofe_car LvlO) LIM_STEPS;
+    
+    om_hl_OP := LocaleOP (Locale := locale heap_lang);
+    om_hl_Degree := ofe_car DegO;
+    om_hl_Level := ofe_car LvlO;
+}.
+Global Existing Instance om_hl_OPRE.
+Global Existing Instance om_hl_OP.
+
+Class OM_HL_Env `(OP: OP_HL DegO LvlO LIM_STEPS)
+  `(EM: ExecutionModel heap_lang M) (Σ: gFunctors):= {
+    ohe_oGS' : @asem_GS _ _ ObligationsASEM Σ;
+    ohe_hGS :: heapGS Σ EM;
+
+    ohe_obls_AMU : @AMU_lift_MU _ _ _ ohe_oGS' _ EM ohe_hGS (↑ nroot);
+    ohe_obls_AMU__f : forall τ, @AMU_lift_MU__f _ _ _ τ ohe_oGS' _ EM _ ⊤;
+    
+    ohe_oGS :: ObligationsGS Σ := ohe_oGS';
+}.
+Global Existing Instance ohe_oGS.
+Global Existing Instance ohe_hGS.
